src/SizeClass.fsti
@@ -1,0 +1,186 @@
+module SizeClass
+
+module US = FStar.SizeT
+module U64 = FStar.UInt64
+module U32 = FStar.UInt32
+module U8 = FStar.UInt8
+
+module A = Steel.Array
+module R = Steel.Reference
+module AL = ArrayList
+
+open Steel.Effect.Atomic
+open Steel.Effect
+
+open Constants
+open Config
+open Utils2
+
+noeq
+type size_class_struct' = {
+  size: sc_union;
+  is_extended: bool;
+  slabs_idxs: A.array US.t;
+  md_count: R.ref US.t;
+  slab_region: array U8.t;
+  md_bm_region: array U64.t;
+  md_bm_region_b: array bool;
+  md_region: array AL.cell;
+}
+
+inline_for_extraction noextract
+let slab_region_size = SlabsCommon2.slab_region_size
+
+inline_for_extraction noextract
+let metadata_max_ex = SlabsCommon2.metadata_max_ex
+
+inline_for_extraction noextract
+let slab_size = SlabsCommon2.slab_size
+
+open FStar.Mul
+type size_class_struct = s:size_class_struct'{
+  array_u8_alignment s.slab_region page_size /\
+  A.length s.slab_region == US.v slab_region_size /\
+  A.length s.slabs_idxs == 7 /\
+  // prove equivalence
+  (s.is_extended ==> (
+    Sc_ex? s.size /\
+    s.md_bm_region == A.null #U64.t /\
+    A.length s.md_bm_region_b == US.v metadata_max_ex/\
+    A.length s.md_region == US.v metadata_max_ex
+  )) /\
+  (not s.is_extended ==> (
+    Sc? s.size /\
+    s.md_bm_region_b == A.null #bool /\
+    A.length s.md_bm_region == US.v metadata_max * 4 /\
+    A.length s.md_region == US.v metadata_max
+  ))
+}
+
+open SteelVRefineDep
+
+unfold
+type size_class_struct_sc = s:size_class_struct{not s.is_extended}
+
+unfold
+type size_class_struct_sc_ex = s:size_class_struct{s.is_extended}
+
+//TODO: should be abstract
+let size_class_vprop_sc
+  (scs: size_class_struct_sc)
+  : vprop
+  =
+  vrefinedep
+    (R.vptr scs.md_count)
+    SlabsCommon.vrefinedep_prop
+    (SlabsCommon.size_class_vprop_aux (get_sc scs.size)
+      scs.slab_region scs.md_bm_region scs.md_region scs.slabs_idxs)
+
+//TODO: should be abstract
+let size_class_vprop_sc_ex
+  (scs: size_class_struct_sc_ex)
+  : vprop
+  =
+  vrefinedep
+    (R.vptr scs.md_count)
+    SlabsCommon2.vrefinedep_prop
+    (SlabsCommon2.size_class_vprop_aux (get_sc_ex scs.size)
+      scs.slab_region scs.md_bm_region_b scs.md_region scs.slabs_idxs)
+
+val size_class_vprop
+  (scs: size_class_struct)
+  : vprop
+
+val size_class_vprop_reveal
+  (scs: size_class_struct)
+  : Lemma
+  (size_class_vprop scs ==
+    (if scs.is_extended
+    then size_class_vprop_sc_ex scs
+    else size_class_vprop_sc scs)
+  )
+
+val allocate_size_class_sc
+  (scs: size_class_struct_sc)
+  : Steel (array U8.t)
+  (size_class_vprop_sc scs)
+  (fun r ->
+    (if (A.is_null r) then emp else A.varray r) `star`
+    size_class_vprop_sc scs)
+  (requires fun h0 -> True)
+  (ensures fun h0 r h1 ->
+    let sc_size = get_sc scs.size in
+    not (A.is_null r) ==> (
+      A.length r == U32.v sc_size /\
+      same_base_array r scs.slab_region /\
+      A.offset (A.ptr_of r) - A.offset (A.ptr_of scs.slab_region) >= 0 /\
+      ((A.offset (A.ptr_of r) - A.offset (A.ptr_of scs.slab_region)) % U32.v page_size) % (U32.v (get_u32 scs.size)) == 0 /\
+      array_u8_alignment r 16ul /\
+      True
+      //((U32.v page_size) % (U32.v scs.size) == 0 ==> array_u8_alignment r scs.size)
+    )
+  )
+
+val deallocate_size_class_sc
+  (scs: size_class_struct_sc)
+  (ptr: array U8.t)
+  (diff: US.t)
+  : Steel bool
+  (A.varray ptr `star`
+  size_class_vprop_sc scs)
+  (fun b ->
+    (if b then emp else A.varray ptr) `star`
+    size_class_vprop_sc scs)
+  (requires fun h0 ->
+    let diff' = A.offset (A.ptr_of ptr) - A.offset (A.ptr_of scs.slab_region) in
+    0 <= diff' /\
+    US.v diff = diff' /\
+    (diff' % U32.v page_size) % U32.v (get_u32 scs.size) == 0 /\
+    A.length ptr == U32.v (get_u32 scs.size) /\
+    same_base_array ptr scs.slab_region)
+  (ensures fun h0 _ h1 -> True)
+
+val allocate_size_class
+  (scs: size_class_struct)
+  : Steel (array U8.t)
+  (size_class_vprop scs)
+  (fun r ->
+    (if (A.is_null r) then emp else A.varray r) `star`
+    size_class_vprop scs)
+  (requires fun h0 -> True)
+  (ensures fun h0 r h1 ->
+    let sc_size = get_u32 scs.size in
+    not (A.is_null r) ==> (
+      A.length r == U32.v sc_size /\
+      same_base_array r scs.slab_region /\
+      A.offset (A.ptr_of r) - A.offset (A.ptr_of scs.slab_region) >= 0 /\
+      //not scs.is_extended ==> ...
+      //scs.is_extended ==> ...
+      //((A.offset (A.ptr_of r) - A.offset (A.ptr_of scs.slab_region)) % U32.v page_size) % (U32.v scs.size) == 0 /\
+      array_u8_alignment r 16ul /\
+      True
+      //((U32.v page_size) % (U32.v scs.size) == 0 ==> array_u8_alignment r scs.size)
+    )
+  )
+
+val deallocate_size_class
+  (scs: size_class_struct)
+  (ptr: array U8.t)
+  (diff: US.t)
+  : Steel bool
+  (A.varray ptr `star`
+  size_class_vprop scs)
+  (fun b ->
+    (if b then emp else A.varray ptr) `star`
+    size_class_vprop scs)
+  (requires fun h0 ->
+    let diff' = A.offset (A.ptr_of ptr) - A.offset (A.ptr_of scs.slab_region) in
+    0 <= diff' /\
+    US.v diff = diff' /\
+    //not scs.is_extended ==> ...
+    //scs.is_extended ==> ...
+    //TODO: to be refined
+    (diff' % U32.v page_size) % U32.v (get_u32 scs.size) == 0 /\
+    A.length ptr == U32.v (get_u32 scs.size) /\
+    same_base_array ptr scs.slab_region)
+  (ensures fun h0 _ h1 -> True)
